proof/invariant-abstract/RISCV64/ArchVSpace_AI.thy
@@ -933,11 +933,11 @@ lemma is_final_cap_caps_of_state_2D:
                         prod_eqI)
   done
 
-crunch underlying_memory[wp]: ackInterrupt, hwASIDFlush, read_sbadaddr, setVSpaceRoot, sfence
+crunch underlying_memory[wp]: ackInterrupt, hwASIDFlush, read_stval, setVSpaceRoot, sfence
   "\<lambda>m'. underlying_memory m' p = um"
   (simp: cache_machine_op_defs machine_op_lift_def machine_rest_lift_def split_def)
 
-crunches storeWord, ackInterrupt, hwASIDFlush, read_sbadaddr, setVSpaceRoot, sfence
+crunches storeWord, ackInterrupt, hwASIDFlush, read_stval, setVSpaceRoot, sfence
   for device_state_inv[wp]: "\<lambda>ms. P (device_state ms)"
   (simp: crunch_simps)
 
